---
title: "Alternating series"
---
An **alternating series** has the form
$$
\sum_{n=0}^\infty (-1)^n a_n,
$$
where typically $a_n\ge 0$.

Some examples:


- For $a_n=n$ we have $\displaystyle\sum_{n=0}^\infty (-1)^n a_n =\sum_{n=0}^\infty (-1)^n n.$
- For $a_n=\frac{1}{n}$ we get the series $\displaystyle \sum_{n=0}^\infty (-1)^n \frac{1}{n}.$

It is easy to see that the first example of an alternating series is not converging, since $\displaystyle\lim_{n\rightarrow\infty }(-1)^na_n$ is not convergent, it is divergent. Now what about the second example? See the figure below.

![Partial sums $s_n$ plotted.](../figures/alternating_series.png){#fig-alternating_series width=70%}


::: {#thm-alt}
**(Alternating Series Test + error bound).**

Let $a_n\ge 0$ be decreasing and $a_n\to 0$. Then $\sum_{n=0}^\infty (-1)^n a_n$ converges.
If $S$ is its sum and $s_n$ the $n$-th partial sum, then
$$
|S-s_n|\le a_{n+1}.
$$
:::

::: {.callout-tip collapse="true" title="Proof"}

Let $b_n=s_{2n}$ and $c_n=s_{2n+1}$. Then for all $n$ we have that $c_n\leq b_n$. Moreover $\{b_n\}$ is decreasing and the elements are bounded below by $c_1$. Also, $\{c_n\}$ is increasing and the elements are bounded above by $b_1$. This means that by the Monotonic Convergence Theorem these sequences are both converging. Also $b_n-c_n=a_{2n+1}\to 0$, so both subsequences have the same limit, hence $S_n\to S$.

Moreover, $|S-s_n|\le |s_{n+1}-s_n| = a_{n+1}.$

:::

::: {.callout-note title="Example"}

Consider the alternating harmonic series
$$
\sum_{n=1}^{\infty}\frac{(-1)^n}{n}.
$$
This is an alternating series, with $a_n=\frac{1}{n}\downarrow 0$. So the series converges. 

In orde to estimate its limit (which is actually $\ln(2)$ as we will see later), we may concentrate on a partial sum. For instance, if we want the error to be less than $0.01$ then it suffices to concentrate on a partial sum $s_n$ such that $a_{n+1}<0.01$. In this case we see that this works if only $\frac{1}{n+1}\leq 0.01$ or $n+1>100 \Leftrightarrow n>99$. So we may take $s_{100}$ as estimate. Below we calculate the partial sum using Python.

```{python}
#| label: alt-harmonic-demo
#| echo: true
#| warning: false
#| message: false   
from IPython.display import display, Math
import math

n = 100
s = sum(((-1)**k)/k for k in range(1, n+1))
S = -math.log(2)
err = abs(S - s)

display(Math(rf"s_{{{n}}} = {s:.10f},\qquad -\ln 2 = {S:.10f},\qquad |S-s_{{{n}}}| = {err:.2e}."))
```


:::